test-asm/check-simple-add.sh
@@ -1,0 +1,9 @@
+#!/bin/sh
+if ../src/ExtractionOCaml/unsaturated_solinas --inline --static --use-value-barrier 25519 64 '(auto)' '2^255 - 19' add \
+  --hints-file simple_avx_add.asm \
+  -o /dev/null --output-asm /dev/null 2>/dev/null; then
+  echo "PASS"
+else
+  echo "FAIL"
+  exit 1
+fi
